Compute assignment targets as seq, not set

src/Verifier/AssignmentTargets.dfy
@@ -1,13 +1,56 @@
 module AssignmentTargets {
   import Ast
+  import opened Basics
 
   export
     provides Compute
     provides Ast
 
-  function Compute(stmt: Ast.Stmt): set<Ast.Variable> {
-    var (vv, cc) := StmtTargets(stmt);
-    if Normal in cc then vv else {}
+  function Compute(stmt: Ast.Stmt): (targets: seq<Ast.Variable>) {
+    var StmtInformation(targets, vv, cc) := StmtTargets(stmt);
+    if Normal in cc then Prune(targets, vv) else []
+  }
+
+  type Target = Ast.Variable
+
+  datatype StmtInformation = StmtInformation(targets: seq<Target>, targetSet: set<Target>, cpoints: set<ContinuationPoint>)
+  {
+    static const EmptyNormal := StmtInformation([], {}, {Normal})
+
+    ghost predicate Valid() {
+      forall target <- targetSet :: target in targets
+    }
+
+    function Add(v: Target): (info: StmtInformation)
+      requires Valid()
+      ensures info.Valid()
+    {
+      if v in targetSet then
+        this
+      else
+        StmtInformation(targets + [v], targetSet + {v}, cpoints)
+    }
+
+    function Remove(v: Target): (info: StmtInformation)
+      requires Valid()
+      ensures info.Valid()
+    {
+      // v stays in the sequence (it is later pruned away by Compute)
+      StmtInformation(targets, targetSet - {v}, cpoints)
+    }
+
+    function AddOutgoingArguments(args: seq<Ast.CallArgument>): (info: StmtInformation)
+      requires Valid()
+      ensures info.Valid()
+      decreases args
+    {
+      if args == [] then
+        this
+      else if args[0].OutgoingArgument? then
+        Add(args[0].v).AddOutgoingArguments(args[1..])
+      else
+        AddOutgoingArguments(args[1..])
+    }
   }
 
   datatype ContinuationPoint =
@@ -18,55 +61,67 @@ module AssignmentTargets {
   // except in those places where control flow is syntactically impossible.
   // To accomplish the latter, the function also returns the set of possible continuation
   // points of `stmt`.
-  function StmtTargets(stmt: Ast.Stmt): (set<Ast.Variable>, set<ContinuationPoint>) {
+  function StmtTargets(stmt: Ast.Stmt): (info: StmtInformation)
+    ensures info.Valid()
+  {
     match stmt
     case VarDecl(v, _, body) =>
-      var (vv, cc) := StmtTargets(body);
-      (vv - {v}, cc)
+      var info := StmtTargets(body);
+      info.Remove(v)
     case Assign(lhs, _) =>
-      ({lhs}, {Normal})
+      StmtInformation([lhs], {lhs}, {Normal})
     case Block(stmts) =>
       BlockTargets(stmts)
     case Call(_, args) =>
-      (set arg <- args | arg.OutgoingArgument? :: arg.v, {Normal})
-    case Check(_) => ({}, {Normal})
-    case Assume(_) => ({}, {Normal})
-    case Assert(_) => ({}, {Normal})
-    case AForall(_, _) => ({}, {Normal})
+      StmtInformation.EmptyNormal.AddOutgoingArguments(args)
+    case Check(_) => StmtInformation.EmptyNormal
+    case Assume(_) => StmtInformation.EmptyNormal
+    case Assert(_) => StmtInformation.EmptyNormal
+    case AForall(_, _) => StmtInformation.EmptyNormal
     case Choose(branches) =>
       ChooseTargets(branches)
     case Loop(_, body) =>
-      var (vv, cc) := StmtTargets(body);
-      (vv, cc - {Normal})
+      var info := StmtTargets(body);
+      info.(cpoints := info.cpoints - {Normal})
     case LabeledStmt(lbl, body) =>
-      var (vv, cc) := StmtTargets(body);
-      if Abrupt(lbl) in cc then
-        (vv, cc - {Abrupt(lbl)} + {Normal})
+      var info := StmtTargets(body);
+      if Abrupt(lbl) in info.cpoints then
+        info.(cpoints := info.cpoints - {Abrupt(lbl)} + {Normal})
       else
-        (vv, cc)
+        info
     case Exit(lbl) =>
-      ({}, {Abrupt(lbl)})
-    case Probe(_) => ({}, {Normal})
+      StmtInformation([], {}, {Abrupt(lbl)})
+    case Probe(_) => StmtInformation.EmptyNormal
   }
 
-  function BlockTargets(stmts: seq<Ast.Stmt>): (set<Ast.Variable>, set<ContinuationPoint>) {
+  function BlockTargets(stmts: seq<Ast.Stmt>): (info: StmtInformation)
+    ensures info.Valid()
+  {
     if stmts == [] then
-      ({}, {Normal})
+      StmtInformation.EmptyNormal
     else
-      var (vv, cc) := StmtTargets(stmts[0]);
-      if Normal in cc then
-        var (vv', cc') := BlockTargets(stmts[1..]);
-        (vv + vv', cc')
+      var info := StmtTargets(stmts[0]);
+      if Normal in info.cpoints then
+        var info' := BlockTargets(stmts[1..]);
+        StmtInformation(
+          info.targets + info'.targets,
+          info.targetSet + info'.targetSet,
+          info.cpoints - {Normal} + info'.cpoints)
       else
-        (vv, cc)
+        info
   }
 
-  function ChooseTargets(stmts: seq<Ast.Stmt>): (set<Ast.Variable>, set<ContinuationPoint>) {
+  function ChooseTargets(stmts: seq<Ast.Stmt>): (info: StmtInformation)
+    ensures info.Valid()
+  {
     if stmts == [] then
-      ({}, {})
+      StmtInformation([], {}, {})
     else
-      var (vv, cc) := StmtTargets(stmts[0]);
-      var (vv', cc') := ChooseTargets(stmts[1..]);
-      (vv + vv', cc + cc')
+      var info := StmtTargets(stmts[0]);
+      var info' := ChooseTargets(stmts[1..]);
+      StmtInformation(
+        info.targets + info'.targets,
+        info.targetSet + info'.targetSet,
+        info.cpoints + info'.cpoints)
   }
 }
